hande recive proof (more or less)

_build/default/src/proofs/funcall/generated_proof_nondent.v.d
@@ -1,2 +1,0 @@
-generated_proof_nondent.vo generated_proof_nondent.glob generated_proof_nondent.v.beautified generated_proof_nondent.required_vo: generated_proof_nondent.v ./generated_code.vo ./generated_spec.vo
-generated_proof_nondent.vio: generated_proof_nondent.v ./generated_code.vio ./generated_spec.vio
