src/solswitch.c
@@ -1,35 +1,38 @@
 #include <stdint.h>
 #include <stdlib.h>
 
+typedef struct [[rc::refined_by("msg: nat")]] ComHandler_t{
+	// uint8_t rxMsg_buf[UNIQUE_MSG_SIZE];
+	// uint8_t rxMsgByteNum;
+	// uint8_t decodedTxMsg_buf[DECODE_MSG_MAX_SIZE];
+    [[rc::field("msg @ int<u8>")]]
+    uint8_t msg;
+
+} ComHandler_t;
+
 typedef  struct
 [[rc::refined_by("state: nat", "msg: nat")]]
 SolenoidSwitchingParams_t{
     [[rc::field("state @ int<size_t>")]]
     size_t state;
-    [[rc::field("msg @ int<size_t>")]]
-    size_t msg;
+    [[rc::field("msg @ ComHandler_t")]]
+    ComHandler_t handler;
 } SolenoidSwitchingParams_t;
 
-//@rc::inlined
-//@Definition SCH_recieveFullMsg_ret (b : nat) : iProp Σ. Admitted. (* TODO: Fill in something here.*)
-//@rc::end
 
-[[rc::parameters("state: nat", "msg: nat", "p: loc")]]
-[[rc::args("p @ &own<{state, msg} @ SolenoidSwitchingParams_t>")]]
+[[rc::parameters("msg: nat", "p: loc")]]
+[[rc::args("p @ &own<{msg} @ ComHandler_t>")]]
 [[rc::exists("new_msg : nat")]]
 [[rc::exists("new_msg_size : nat")]]
 [[rc::returns("new_msg_size @ int<u8>")]]
-[[rc::ensures("own p : {state,new_msg} @ SolenoidSwitchingParams_t")]]
- uint8_t SCH_recieveFullMsg(SolenoidSwitchingParams_t* ssp) { return 2; /* need to return something for proof to work */ }
+[[rc::ensures("own p : {new_msg} @ ComHandler_t")]]
+ uint8_t SCH_recieveFullMsg(ComHandler_t* handler) { return 2; /* need to return something for proof to work */ }
 
 [[rc::parameters("state: nat", "msg: nat", "p: loc")]]
 [[rc::args("p @ &own<{state, msg} @ SolenoidSwitchingParams_t>")]]
 [[rc::exists("new_state : nat")]]
-// [[rc::ensures("own p : { (if Nat.eqb state 0%nat then 1%nat else state) ,msg} @ SolenoidSwitchingParams_t")]]
 [[rc::ensures("own p : { new_state ,msg} @ SolenoidSwitchingParams_t")]]
 [[rc::ensures("{new_state = (if Nat.eqb state 0%nat then 1%nat else state)}")]]
-// [[rc::ensures("{state = 0%nat} @ optional<1%nat,state> @ new_state")]]
-// [[rc::ensures("own p : {state = 0%nat} @ optional<{1%nat,msg} @ SolenoidSwitchingParams_t ,{state,msg} @ SolenoidSwitchingParams_t>")]]
 [[rc::tactics("all: try destruct state. try lia. try auto.")]]
 void SML_switchTheSolenoid( SolenoidSwitchingParams_t* ssp){
 
@@ -48,55 +51,30 @@ void SML_switchTheSolenoid( SolenoidSwitchingParams_t* ssp){
 [[rc::args("p @ &own<{state, msg} @ SolenoidSwitchingParams_t>")]]
 [[rc::exists("new_msg : nat")]]
 [[rc::exists("new_state : nat")]]
-[[rc::exists("new_msg_size : nat")]]
-// [[rc::ensures("own p : { (if Nat.eqb new_msg_size 8%nat then 1%nat else state) ,new_msg} @ SolenoidSwitchingParams_t")]]
-// [[rc::ensures("{((new_msg_size = 8%nat)) -> new_state = 1%nat}")]]
-// [[rc::ensures("[SCH_recieveFullMsg_ret (if new_state is 1%nat then 8%nat else 0%nat)]")]]
 [[rc::ensures("own p : { new_state ,new_msg} @ SolenoidSwitchingParams_t")]]
-//[[rc::ensures("{(new_msg_size = 8%nat) -> (new_state = 1%nat)}")]]
-// [[rc::ensures("{∃ n, (and (new_msg_size = n) (n <> 8%nat)) -> new_state = state}")]]
-[[rc::ensures("{∃ len, or ((len = 8%nat) -> (new_state = 1%nat)) ((len <> 8%nat) -> (new_state = state))}")]]
-[[rc::tactics("exists 8%nat. left. auto." )]]
+//inorder to reason about the nondent value of `SCH_recieveFullMsg` we need to add an ∃ len, otherwise refinedc can unify a value for it.
+//so in order to complete the proof we have to provide values for each case (and else case).
+[[rc::ensures("{∃ len, ((new_msg = 7%nat ∨ new_msg = 12%nat) ∧ (len = 8%nat) ∧ (state = 0%nat) -> (new_state = 1%nat)) ∨ ((len <> 8%nat) -> (new_state = state))}")]]
+[[rc::tactics("exists 8%nat. left. auto. intros [_ [_ HH1]]. rewrite HH1. auto." )]]
+[[rc::tactics("exists 8%nat. left. auto. intros [_ [_ HH1]]. rewrite HH1. auto." )]]
+[[rc::tactics("exists 0%nat. right. auto. " )]]
 [[rc::tactics("exists 0%nat. right. auto. " )]]
 [[rc::tactics("exists 0%nat. right. auto. " )]]
 void SML_handleReceivedMsgs(SolenoidSwitchingParams_t* ssp)
 {
-    uint8_t rxMsgSize = SCH_recieveFullMsg(ssp);
+    uint8_t rxMsgSize = SCH_recieveFullMsg(&ssp->handler);
     if(rxMsgSize != INVALID_MSG_SIZE){
         if(rxMsgSize == UNIQUE_MSG_SIZE){
-            //if(ssp->msg == UNIQUE_MSG_A /*|| ssp->msg == UNIQUE_MSG_B*/){ // todo - msg should be array. not supported in refinedc?
-               //SML_switchTheSolenoid(ssp);
-            //}
-            ssp->state = 1;
+            if(ssp->handler.msg == UNIQUE_MSG_A || ssp->handler.msg == UNIQUE_MSG_B){ // todo - msg should be array.
+               SML_switchTheSolenoid(ssp);
+            }
         }
     }
-    
 }
 
-// [[rc::parameters("state: nat", "msg: nat", "p: loc", "len: nat")]]
-// [[rc::args("p @ &own<{state, msg} @ SolenoidSwitchingParams_t>", "len @ int<u8>")]]
-// [[rc::exists("new_msg : nat")]]
-// [[rc::exists("new_state : nat")]]
-// [[rc::ensures("own p : { new_state ,new_msg} @ SolenoidSwitchingParams_t")]]
-// [[rc::ensures("{or (and (len = 8%nat) (new_state = 1%nat)) (and (len <> 8%nat) (new_state = state))}")]]
-// //[[rc::ensures("{new_state = 1%nat ∨ new_state = state}")]]
-// void SML_handleReceivedMsgs_with_length(SolenoidSwitchingParams_t* ssp, uint8_t rxMsgSize)
-// {
-//     // if(rxMsgSize != INVALID_MSG_SIZE){
-//         if(rxMsgSize == UNIQUE_MSG_SIZE){
-//             //if(ssp->msg == UNIQUE_MSG_A /*|| ssp->msg == UNIQUE_MSG_B*/){ // todo - msg should be array. not supported in refinedc?
-//                //SML_switchTheSolenoid(ssp);
-//             //}
-//             ssp->state = 1;
-//         }
-//     // }
-    
-// }
-
-
-
-// void SML_handleReceivedMsgs(SolenoidSwitchingParams_t* ssp)
-// {
-//     uint8_t rxMsgSize = SCH_recieveFullMsg(ssp);
-//     SML_handleReceivedMsgs_with_length(ssp, rxMsgSize);
-// }
+/*
+→
+∧
+∨
+∃
+*/
