_build/default/src/proofs/funcall/generated_code.v
@@ -5,21 +5,6 @@ Set Default Proof Using "Type".
 
 (* Generated from [src/funcall.c]. *)
 Section code.
-  Definition file_0 : string := "src/funcall.c".
-  Definition loc_2 : location_info := LocationInfo file_0 22 19 22 28.
-  Definition loc_3 : location_info := LocationInfo file_0 22 26 22 27.
-  Definition loc_6 : location_info := LocationInfo file_0 29 4 31 5.
-  Definition loc_7 : location_info := LocationInfo file_0 32 4 32 13.
-  Definition loc_8 : location_info := LocationInfo file_0 32 11 32 12.
-  Definition loc_9 : location_info := LocationInfo file_0 29 22 31 5.
-  Definition loc_10 : location_info := LocationInfo file_0 30 8 30 17.
-  Definition loc_11 : location_info := LocationInfo file_0 30 15 30 16.
-  Definition loc_12 : location_info := LocationInfo file_0 29 4 31 5.
-  Definition loc_13 : location_info := LocationInfo file_0 29 7 29 21.
-  Definition loc_14 : location_info := LocationInfo file_0 29 7 29 16.
-  Definition loc_15 : location_info := LocationInfo file_0 29 7 29 14.
-  Definition loc_16 : location_info := LocationInfo file_0 29 7 29 14.
-  Definition loc_17 : location_info := LocationInfo file_0 29 20 29 21.
 
   (* Definition of struct [div]. *)
   Program Definition struct_div := {|
@@ -48,51 +33,19 @@ Section code.
   |}.
   Solve Obligations with solve_struct_obligations.
 
-  (* Definition of function [nondent]. *)
-  Definition impl_nondent : function := {|
-    f_args := [
+  (* Definition of struct [ComHandler]. *)
+  Program Definition struct_ComHandler := {|
+    sl_members := [
+      (Some "msg", it_layout u8)
     ];
-    f_local_vars := [
-    ];
-    f_init := "#0";
-    f_code := (
-      <[ "#0" :=
-        locinfo: loc_2 ;
-        Return (LocInfoE loc_3 (UnOp (CastOp $ BoolOp) (IntOp i32) (LocInfoE loc_3 (i2v 2 i32))))
-      ]> $∅
-    )%E
   |}.
+  Solve Obligations with solve_struct_obligations.
 
-  (* Definition of function [foo]. *)
-  Definition impl_foo (global_nondent : loc): function := {|
-    f_args := [
+  (* Definition of struct [MyStruct]. *)
+  Program Definition struct_MyStruct := {|
+    sl_members := [
+      (Some "cmdhandler", layout_of struct_ComHandler)
     ];
-    f_local_vars := [
-    ];
-    f_init := "#0";
-    f_code := (
-      <[ "#0" :=
-        locinfo: loc_13 ;
-        if{IntOp i32}: LocInfoE loc_13 ((LocInfoE loc_14 (UnOp (CastOp $ IntOp i32) (BoolOp) (LocInfoE loc_14 (Call (LocInfoE loc_16 (global_nondent)) [@{expr}  ])))) ={IntOp i32, IntOp i32, i32} (LocInfoE loc_17 (i2v 2 i32)))
-        then
-        locinfo: loc_10 ;
-          Goto "#2"
-        else
-        locinfo: loc_7 ;
-          Goto "#3"
-      ]> $
-      <[ "#1" :=
-        locinfo: loc_7 ;
-        Return (LocInfoE loc_8 (i2v 2 i32))
-      ]> $
-      <[ "#2" :=
-        locinfo: loc_10 ;
-        Return (LocInfoE loc_11 (i2v 1 i32))
-      ]> $
-      <[ "#3" :=
-        locinfo: loc_7 ;
-        Goto "#1"
-      ]> $∅
-    )%E
   |}.
+  Solve Obligations with solve_struct_obligations.
 End code.
