_build/default/src/proofs/solswitch/generated_code.v
@@ -6,47 +6,67 @@ Set Default Proof Using "Type".
 (* Generated from [src/solswitch.c]. *)
 Section code.
   Definition file_0 : string := "src/solswitch.c".
-  Definition loc_2 : location_info := LocationInfo file_0 23 62 23 71.
-  Definition loc_3 : location_info := LocationInfo file_0 23 69 23 70.
-  Definition loc_6 : location_info := LocationInfo file_0 36 1 39 2.
-  Definition loc_7 : location_info := LocationInfo file_0 36 23 39 2.
-  Definition loc_8 : location_info := LocationInfo file_0 38 2 38 17.
-  Definition loc_9 : location_info := LocationInfo file_0 38 2 38 12.
-  Definition loc_10 : location_info := LocationInfo file_0 38 2 38 5.
-  Definition loc_11 : location_info := LocationInfo file_0 38 2 38 5.
-  Definition loc_12 : location_info := LocationInfo file_0 38 15 38 16.
-  Definition loc_13 : location_info := LocationInfo file_0 36 1 39 2.
-  Definition loc_14 : location_info := LocationInfo file_0 36 6 36 21.
-  Definition loc_15 : location_info := LocationInfo file_0 36 6 36 7.
-  Definition loc_16 : location_info := LocationInfo file_0 36 11 36 21.
-  Definition loc_17 : location_info := LocationInfo file_0 36 11 36 21.
-  Definition loc_18 : location_info := LocationInfo file_0 36 11 36 14.
-  Definition loc_19 : location_info := LocationInfo file_0 36 11 36 14.
-  Definition loc_22 : location_info := LocationInfo file_0 64 4 64 48.
-  Definition loc_23 : location_info := LocationInfo file_0 65 4 72 5.
-  Definition loc_24 : location_info := LocationInfo file_0 65 22 72 5.
-  Definition loc_25 : location_info := LocationInfo file_0 66 8 71 9.
-  Definition loc_26 : location_info := LocationInfo file_0 66 26 71 9.
-  Definition loc_27 : location_info := LocationInfo file_0 70 12 70 27.
-  Definition loc_28 : location_info := LocationInfo file_0 70 12 70 22.
-  Definition loc_29 : location_info := LocationInfo file_0 70 12 70 15.
-  Definition loc_30 : location_info := LocationInfo file_0 70 12 70 15.
-  Definition loc_31 : location_info := LocationInfo file_0 70 25 70 26.
-  Definition loc_32 : location_info := LocationInfo file_0 66 8 71 9.
-  Definition loc_33 : location_info := LocationInfo file_0 66 11 66 25.
-  Definition loc_34 : location_info := LocationInfo file_0 66 11 66 20.
-  Definition loc_35 : location_info := LocationInfo file_0 66 11 66 20.
-  Definition loc_36 : location_info := LocationInfo file_0 66 24 66 25.
-  Definition loc_37 : location_info := LocationInfo file_0 65 4 72 5.
-  Definition loc_38 : location_info := LocationInfo file_0 65 7 65 21.
-  Definition loc_39 : location_info := LocationInfo file_0 65 7 65 16.
-  Definition loc_40 : location_info := LocationInfo file_0 65 7 65 16.
-  Definition loc_41 : location_info := LocationInfo file_0 65 20 65 21.
-  Definition loc_42 : location_info := LocationInfo file_0 64 24 64 47.
-  Definition loc_43 : location_info := LocationInfo file_0 64 24 64 42.
-  Definition loc_44 : location_info := LocationInfo file_0 64 24 64 42.
-  Definition loc_45 : location_info := LocationInfo file_0 64 43 64 46.
-  Definition loc_46 : location_info := LocationInfo file_0 64 43 64 46.
+  Definition loc_2 : location_info := LocationInfo file_0 31 53 31 62.
+  Definition loc_3 : location_info := LocationInfo file_0 31 60 31 61.
+  Definition loc_6 : location_info := LocationInfo file_0 41 1 44 2.
+  Definition loc_7 : location_info := LocationInfo file_0 41 23 44 2.
+  Definition loc_8 : location_info := LocationInfo file_0 43 2 43 17.
+  Definition loc_9 : location_info := LocationInfo file_0 43 2 43 12.
+  Definition loc_10 : location_info := LocationInfo file_0 43 2 43 5.
+  Definition loc_11 : location_info := LocationInfo file_0 43 2 43 5.
+  Definition loc_12 : location_info := LocationInfo file_0 43 15 43 16.
+  Definition loc_13 : location_info := LocationInfo file_0 41 1 44 2.
+  Definition loc_14 : location_info := LocationInfo file_0 41 6 41 21.
+  Definition loc_15 : location_info := LocationInfo file_0 41 6 41 7.
+  Definition loc_16 : location_info := LocationInfo file_0 41 11 41 21.
+  Definition loc_17 : location_info := LocationInfo file_0 41 11 41 21.
+  Definition loc_18 : location_info := LocationInfo file_0 41 11 41 14.
+  Definition loc_19 : location_info := LocationInfo file_0 41 11 41 14.
+  Definition loc_22 : location_info := LocationInfo file_0 65 4 65 58.
+  Definition loc_23 : location_info := LocationInfo file_0 66 4 72 5.
+  Definition loc_24 : location_info := LocationInfo file_0 66 22 72 5.
+  Definition loc_25 : location_info := LocationInfo file_0 67 8 71 9.
+  Definition loc_26 : location_info := LocationInfo file_0 67 26 71 9.
+  Definition loc_27 : location_info := LocationInfo file_0 68 12 70 13.
+  Definition loc_28 : location_info := LocationInfo file_0 68 63 70 13.
+  Definition loc_29 : location_info := LocationInfo file_0 69 15 69 42.
+  Definition loc_30 : location_info := LocationInfo file_0 69 15 69 36.
+  Definition loc_31 : location_info := LocationInfo file_0 69 15 69 36.
+  Definition loc_32 : location_info := LocationInfo file_0 69 37 69 40.
+  Definition loc_33 : location_info := LocationInfo file_0 69 37 69 40.
+  Definition loc_34 : location_info := LocationInfo file_0 68 12 70 13.
+  Definition loc_35 : location_info := LocationInfo file_0 68 15 68 62.
+  Definition loc_36 : location_info := LocationInfo file_0 68 15 68 36.
+  Definition loc_37 : location_info := LocationInfo file_0 68 15 68 31.
+  Definition loc_38 : location_info := LocationInfo file_0 68 15 68 31.
+  Definition loc_39 : location_info := LocationInfo file_0 68 15 68 27.
+  Definition loc_40 : location_info := LocationInfo file_0 68 15 68 18.
+  Definition loc_41 : location_info := LocationInfo file_0 68 15 68 18.
+  Definition loc_42 : location_info := LocationInfo file_0 68 35 68 36.
+  Definition loc_43 : location_info := LocationInfo file_0 68 40 68 62.
+  Definition loc_44 : location_info := LocationInfo file_0 68 40 68 56.
+  Definition loc_45 : location_info := LocationInfo file_0 68 40 68 56.
+  Definition loc_46 : location_info := LocationInfo file_0 68 40 68 52.
+  Definition loc_47 : location_info := LocationInfo file_0 68 40 68 43.
+  Definition loc_48 : location_info := LocationInfo file_0 68 40 68 43.
+  Definition loc_49 : location_info := LocationInfo file_0 68 60 68 62.
+  Definition loc_50 : location_info := LocationInfo file_0 67 8 71 9.
+  Definition loc_51 : location_info := LocationInfo file_0 67 11 67 25.
+  Definition loc_52 : location_info := LocationInfo file_0 67 11 67 20.
+  Definition loc_53 : location_info := LocationInfo file_0 67 11 67 20.
+  Definition loc_54 : location_info := LocationInfo file_0 67 24 67 25.
+  Definition loc_55 : location_info := LocationInfo file_0 66 4 72 5.
+  Definition loc_56 : location_info := LocationInfo file_0 66 7 66 21.
+  Definition loc_57 : location_info := LocationInfo file_0 66 7 66 16.
+  Definition loc_58 : location_info := LocationInfo file_0 66 7 66 16.
+  Definition loc_59 : location_info := LocationInfo file_0 66 20 66 21.
+  Definition loc_60 : location_info := LocationInfo file_0 65 24 65 57.
+  Definition loc_61 : location_info := LocationInfo file_0 65 24 65 42.
+  Definition loc_62 : location_info := LocationInfo file_0 65 24 65 42.
+  Definition loc_63 : location_info := LocationInfo file_0 65 43 65 56.
+  Definition loc_64 : location_info := LocationInfo file_0 65 44 65 56.
+  Definition loc_65 : location_info := LocationInfo file_0 65 44 65 47.
+  Definition loc_66 : location_info := LocationInfo file_0 65 44 65 47.
 
   (* Definition of struct [div]. *)
   Program Definition struct_div := {|
@@ -75,11 +95,20 @@ Section code.
   |}.
   Solve Obligations with solve_struct_obligations.
 
+  (* Definition of struct [ComHandler_t]. *)
+  Program Definition struct_ComHandler_t := {|
+    sl_members := [
+      (Some "msg", it_layout u8)
+    ];
+  |}.
+  Solve Obligations with solve_struct_obligations.
+
   (* Definition of struct [SolenoidSwitchingParams_t]. *)
   Program Definition struct_SolenoidSwitchingParams_t := {|
     sl_members := [
       (Some "state", it_layout size_t);
-      (Some "msg", it_layout size_t)
+      (Some "handler", layout_of struct_ComHandler_t);
+      (None, Layout 7%nat 0%nat)
     ];
   |}.
   Solve Obligations with solve_struct_obligations.
@@ -87,7 +116,7 @@ Section code.
   (* Definition of function [SCH_recieveFullMsg]. *)
   Definition impl_SCH_recieveFullMsg : function := {|
     f_args := [
-      ("ssp", void*)
+      ("handler", void*)
     ];
     f_local_vars := [
     ];
@@ -131,7 +160,7 @@ Section code.
   |}.
 
   (* Definition of function [SML_handleReceivedMsgs]. *)
-  Definition impl_SML_handleReceivedMsgs (global_SCH_recieveFullMsg : loc): function := {|
+  Definition impl_SML_handleReceivedMsgs (global_SCH_recieveFullMsg global_SML_switchTheSolenoid : loc): function := {|
     f_args := [
       ("ssp", void*)
     ];
@@ -142,34 +171,45 @@ Section code.
     f_code := (
       <[ "#0" :=
         "rxMsgSize" <-{ IntOp u8 }
-          LocInfoE loc_42 (Call (LocInfoE loc_44 (global_SCH_recieveFullMsg)) [@{expr} LocInfoE loc_45 (use{PtrOp} (LocInfoE loc_46 ("ssp"))) ]) ;
-        locinfo: loc_38 ;
-        if{IntOp i32}: LocInfoE loc_38 ((LocInfoE loc_39 (UnOp (CastOp $ IntOp i32) (IntOp u8) (LocInfoE loc_39 (use{IntOp u8} (LocInfoE loc_40 ("rxMsgSize")))))) !={IntOp i32, IntOp i32, i32} (LocInfoE loc_41 (i2v 0 i32)))
+          LocInfoE loc_60 (Call (LocInfoE loc_62 (global_SCH_recieveFullMsg)) [@{expr} LocInfoE loc_63 (&(LocInfoE loc_64 ((LocInfoE loc_65 (!{PtrOp} (LocInfoE loc_66 ("ssp")))) at{struct_SolenoidSwitchingParams_t} "handler"))) ]) ;
+        locinfo: loc_56 ;
+        if{IntOp i32}: LocInfoE loc_56 ((LocInfoE loc_57 (UnOp (CastOp $ IntOp i32) (IntOp u8) (LocInfoE loc_57 (use{IntOp u8} (LocInfoE loc_58 ("rxMsgSize")))))) !={IntOp i32, IntOp i32, i32} (LocInfoE loc_59 (i2v 0 i32)))
         then
-        locinfo: loc_33 ;
+        locinfo: loc_51 ;
           Goto "#1"
+        else
+        Goto "#6"
+      ]> $
+      <[ "#1" :=
+        locinfo: loc_51 ;
+        if{IntOp i32}: LocInfoE loc_51 ((LocInfoE loc_52 (UnOp (CastOp $ IntOp i32) (IntOp u8) (LocInfoE loc_52 (use{IntOp u8} (LocInfoE loc_53 ("rxMsgSize")))))) ={IntOp i32, IntOp i32, i32} (LocInfoE loc_54 (i2v 8 i32)))
+        then
+        locinfo: loc_35 ;
+          Goto "#2"
+        else
+        Goto "#5"
+      ]> $
+      <[ "#2" :=
+        locinfo: loc_35 ;
+        if{IntOp i32}: LocInfoE loc_35 ((LocInfoE loc_36 ((LocInfoE loc_37 (UnOp (CastOp $ IntOp i32) (IntOp u8) (LocInfoE loc_37 (use{IntOp u8} (LocInfoE loc_38 ((LocInfoE loc_39 ((LocInfoE loc_40 (!{PtrOp} (LocInfoE loc_41 ("ssp")))) at{struct_SolenoidSwitchingParams_t} "handler")) at{struct_ComHandler_t} "msg")))))) ={IntOp i32, IntOp i32, i32} (LocInfoE loc_42 (i2v 7 i32)))) ||{IntOp i32, IntOp i32, i32} (LocInfoE loc_43 ((LocInfoE loc_44 (UnOp (CastOp $ IntOp i32) (IntOp u8) (LocInfoE loc_44 (use{IntOp u8} (LocInfoE loc_45 ((LocInfoE loc_46 ((LocInfoE loc_47 (!{PtrOp} (LocInfoE loc_48 ("ssp")))) at{struct_SolenoidSwitchingParams_t} "handler")) at{struct_ComHandler_t} "msg")))))) ={IntOp i32, IntOp i32, i32} (LocInfoE loc_49 (i2v 12 i32)))))
+        then
+        locinfo: loc_29 ;
+          Goto "#3"
         else
         Goto "#4"
       ]> $
-      <[ "#1" :=
-        locinfo: loc_33 ;
-        if{IntOp i32}: LocInfoE loc_33 ((LocInfoE loc_34 (UnOp (CastOp $ IntOp i32) (IntOp u8) (LocInfoE loc_34 (use{IntOp u8} (LocInfoE loc_35 ("rxMsgSize")))))) ={IntOp i32, IntOp i32, i32} (LocInfoE loc_36 (i2v 8 i32)))
-        then
-        locinfo: loc_27 ;
-          Goto "#2"
-        else
-        Goto "#3"
-      ]> $
-      <[ "#2" :=
-        locinfo: loc_27 ;
-        LocInfoE loc_28 ((LocInfoE loc_29 (!{PtrOp} (LocInfoE loc_30 ("ssp")))) at{struct_SolenoidSwitchingParams_t} "state") <-{ IntOp size_t }
-          LocInfoE loc_31 (UnOp (CastOp $ IntOp size_t) (IntOp i32) (LocInfoE loc_31 (i2v 1 i32))) ;
-        Return (VOID)
-      ]> $
       <[ "#3" :=
+        locinfo: loc_29 ;
+        expr: (LocInfoE loc_29 (Call (LocInfoE loc_31 (global_SML_switchTheSolenoid)) [@{expr} LocInfoE loc_32 (use{PtrOp} (LocInfoE loc_33 ("ssp"))) ])) ;
         Return (VOID)
       ]> $
       <[ "#4" :=
+        Return (VOID)
+      ]> $
+      <[ "#5" :=
+        Return (VOID)
+      ]> $
+      <[ "#6" :=
         Return (VOID)
       ]> $∅
     )%E
